Update file2.dfy

file2.dfy
@@ -24,7 +24,8 @@ predicate isOptSol(sol : seq<int>, nr:int)
     requires sol[2]>=0
 {   
   isSol(sol,nr) &&
-  forall sol' :: |sol'| == 3 && sol'[0]>=0 && sol'[1]>=0 && sol'[2]>=0 && isSol(sol',nr) ==> cost(sol') >= cost(sol)
+  forall sol' :: |sol'| == 3 && sol'[0]>=0 && sol'[1]>=0 && sol'[2]>=0 && isSol(sol',nr) 
+          ==> cost(sol') >= cost(sol)
 
 }
 
@@ -33,9 +34,11 @@ predicate INV(copie: int, nr: int, s1: int, s5: int, s10:int)
   requires s5 >= 0
   requires s10 >= 0
 {
-   forall s1', s5', s10' :: s1'>=0 && s5'>=0 && s10'>=0 
-          && isOptSol([s1',s5',s10'],copie) ==> 
-          isOptSol([s1+s1',s5+s5',s10+s10'],nr)
+   forall s1', s5', s10' :: s1'>=0 && s5'>=0 && s10'>=0 ==>
+          (isSol([s1',s5',s10'],copie) ==> 
+          isSol([s1+s1',s5+s5',s10+s10'],nr)) &&
+          (isOptSol([s1',s5',s10'],copie) ==> 
+          isOptSol([s1+s1',s5+s5',s10+s10'],nr))
 }
 
 
@@ -44,6 +47,8 @@ method findMax(nr: int) returns(s:int)
   ensures 0 < s <= nr
   ensures s == 1 || s == 5 || s == 10
   ensures s == 1 ==> nr < 5
+  ensures s == 5 ==> nr >= 5
+  ensures s == 10 ==> nr >=10
   
 {
   if(nr >= 10){
@@ -67,7 +72,28 @@ lemma caz1(copie: int, nr: int, s1: int, s5: int, s10: int)
   requires INV(copie,nr,s1,s5,s10)
   ensures INV(copie-1,nr,s1+1,s5,s10)
 {
-  assume false;
+
+  forall s1', s5', s10' | s1'>=0 && s5'>=0 && s10'>=0 
+          && isOptSol([s1',s5',s10'],copie-1) 
+          ensures isOptSol([s1+s1'+1,s5+s5',s10+s10'],nr)
+  {
+    assert isSol([s1',s5',s10'],copie-1);
+    assert isSol([s1'+1,s5',s10'],copie);
+
+    assert forall sol' :: |sol'| == 3 && sol'[0]>=0 && sol'[1]>=0 && sol'[2]>=0 
+          && isSol(sol',copie-1) 
+          ==> cost(sol') >= cost([s1',s5',s10']);
+    assert isSol([s1+s1'+1,s5+s5',s10+s10'],nr);
+    assert forall sol' :: |sol'| == 3 && sol'[0]>=0 && sol'[1]>=0 && sol'[2]>=0 
+          && isSol(sol',nr) 
+          ==> cost(sol') >= cost([s1+s1'+1,s5+s5',s10+s10']);
+  }
+
+  assert forall s1', s5', s10' :: s1'>=0 && s5'>=0 && s10'>=0 
+          && isOptSol([s1',s5',s10'],copie-1) ==> 
+          isOptSol([s1+s1'+1,s5+s5',s10+s10'],nr);
+  
+
 }
 
 lemma caz2(copie: int,nr: int,s1: int,s5: int,s10: int)
@@ -78,7 +104,25 @@ lemma caz2(copie: int,nr: int,s1: int,s5: int,s10: int)
   requires INV(copie,nr,s1,s5,s10)
   ensures INV(copie-5,nr,s1,s5+1,s10)
 {
-  assume false;
+
+ forall s1', s5', s10' | s1'>=0 && s5'>=0 && s10'>=0 
+          && isOptSol([s1',s5',s10'],copie-5) 
+          ensures isOptSol([s1+s1',s5+s5'+1,s10+s10'],nr)
+  {
+    assert isSol([s1',s5',s10'],copie-5);
+    assert isSol([s1',s5'+1,s10'],copie);
+
+    assert forall sol' :: |sol'| == 3 && sol'[0]>=0 && sol'[1]>=0 && sol'[2]>=0 && isSol(sol',copie-5) 
+          ==> cost(sol') >= cost([s1',s5',s10']);
+    assert isSol([s1+s1',s5+s5'+1,s10+s10'],nr);
+    assert forall sol' :: |sol'| == 3 && sol'[0]>=0 && sol'[1]>=0 && sol'[2]>=0 && isSol(sol',nr) 
+          ==> cost(sol') >= cost([s1+s1',s5+s5'+1,s10+s10']);
+  }
+
+  assert forall s1', s5', s10' :: s1'>=0 && s5'>=0 && s10'>=0 
+          && isOptSol([s1',s5',s10'],copie-5) ==> 
+          isOptSol([s1+s1',s5+s5'+1,s10+s10'],nr);
+
 }
 
 lemma caz3(copie: int,nr: int,s1: int,s5: int,s10: int)
@@ -90,6 +134,24 @@ lemma caz3(copie: int,nr: int,s1: int,s5: int,s10: int)
   ensures INV(copie-10,nr,s1,s5,s10+1)
 {
   assume false;
+  // forall s1', s5', s10' | s1'>=0 && s5'>=0 && s10'>=0 
+  //         && isOptSol([s1',s5',s10'],copie-10) 
+  //         ensures isOptSol([s1+s1',s5+s5',s10+s10'+1],nr)
+  // {
+  //   assert isSol([s1',s5',s10'],copie-10);
+  //   assert isSol([s1',s5',s10'+1],copie);
+
+  //   assert forall sol' :: |sol'| == 3 && sol'[0]>=0 && sol'[1]>=0 && sol'[2]>=0 
+  //         && isSol(sol',copie-10) 
+  //         ==> cost(sol') >= cost([s1',s5',s10']);
+  //   assert isSol([s1+s1',s5+s5',s10+s10'+1],nr);
+  //   assert forall sol' :: |sol'| == 3 && sol'[0]>=0 && sol'[1]>=0 && sol'[2]>=0 && isSol(sol',nr) 
+  //         ==> cost(sol') >= cost([s1+s1',s5+s5',s10+s10'+1]);
+  // }
+
+  // assert forall s1', s5', s10' :: s1'>=0 && s5'>=0 && s10'>=0 
+  //         && isOptSol([s1',s5',s10'],copie-10) ==> 
+  //         isOptSol([s1+s1',s5+s5',s10+s10'+1],nr);
 }
 
 
@@ -140,7 +202,6 @@ lemma caz3(copie: int,nr: int,s1: int,s5: int,s10: int)
         copie := copie-s;
     }
     sol := [s1,s5,s10];
-
   }
 
   
